

Ahhh, I got you! Don't worry — we can go **super slowly**, no math fear here 😊. Let's break it down **step by step** with very simple numbers.

We want to see **why** this line:

```
cpp

ans = ans * (nRow - i) / i;
```

is just the combination formula in disguise.

---

## 1 Start with the combination formula

The combination formula is:

$$C(n, r) = \frac{n!}{r!(n - r)!}$$

This tells you: "How many ways can I choose  $r$  items from  $n$  items?"

---

## 2 Look at consecutive numbers in a row

Suppose we are in **row  $n = 4$**  (which is the 5th row in 1-based indexing):

$$C(4, 0), C(4, 1), C(4, 2), C(4, 3), C(4, 4)$$

We know:

- $C(4, 0) = 1$
  - $C(4, 1) = 4$
  - $C(4, 2) = 6$
  - $C(4, 3) = 4$
  - $C(4, 4) = 1$
- 

### Step 2a — Write formulas

$$C(4, 1) = \frac{4!}{1! \cdot 3!} = \frac{24}{6} = 4$$

$$C(4, 2) = \frac{4!}{2! \cdot 2!} = \frac{24}{4} = 6$$

$$C(4, 3) = \frac{4!}{3! \cdot 1!} = \frac{24}{6} = 4$$

## Step 2b — Notice a pattern

Let's try to get **C(4,1)** from **C(4,0)**:

$$C(4, 0) = 1$$

$$C(4, 1) = C(4, 0) \times \frac{4 - 0}{1} = 1 \times \frac{4}{1} = 4$$

✓ Works!

Next, **C(4,2)** from **C(4,1)**:

$$C(4, 2) = C(4, 1) \times \frac{4 - 1}{2} = 4 \times \frac{3}{2} = 6$$

Next, **C(4,3)** from **C(4,2)**:

$$C(4, 3) = C(4, 2) \times \frac{4 - 2}{3} = 6 \times \frac{2}{3} = 4$$

Next, **C(4,4)** from **C(4,3)**:

$$C(4, 4) = C(4, 3) \times \frac{4 - 3}{4} = 4 \times \frac{1}{4} = 1$$

🎉 Works every time.

## 3 Connect to your code

In your code:

```
cpp
ans = ans * (nRow - i) / i;
```

- **ans** → stores **previous combination**, i.e.,  $C(n, r-1)$
- **i** → is **r** in  $C(n, r)$
- **nRow** → is **row length**, which is **n+1** (because the code counts 1-based)

So effectively:

$$C(n, r) = C(n, r - 1) \times \frac{n - (r - 1)}{r} = C(n, r - 1) \times \frac{n - r + 1}{r}$$

✓ That's exactly what the code does.